progress

proofs/x86-64/avx2/ml_dsa_65/row_vector.ec
@@ -97,27 +97,97 @@ wp; call polynomial__pointwise_montgomery_multiply_and_reduce_ll.
 by auto => /#.
 qed.
 
+op dotp_partial (v1 v2 : polylvec) (k : int) : poly =
+  foldr (fun (i : int) (a : poly) => (basemul v1.[i] v2.[i]) &+ a)
+        poly_zero (iota_ 0 k).
+
+lemma dotp_partialS (v1 v2 : polylvec) (k : int) :
+  0 <= k => dotp_partial v1 v2 (k + 1) = basemul v1.[k] v2.[k] &+ dotp_partial v1 v2 k.
+proof. admitted. (* todo algebra PY *)
+
+lemma dotp_partial_ntt_dotp (v1 v2 : polylvec) :
+  dotp_partial v1 v2 lvec = ntt_dotp v1 v2.
+proof. by rewrite /dotp_partial /ntt_dotp. qed.
+
 lemma row_vector____dot_product_correct
       (_out : W32.t Array256.t)
       (_lhs : W32.t Array1280.t) (_rhs : W32.t Array1280.t) :
     hoare [ M.row_vector____dot_product :
         output = _out /\ lhs = _lhs /\ rhs = _rhs /\
-        wpolylvec_ntt_orng (lvec_unflatten256 _lhs) /\
-        wpolylvec_ntt_orng (lvec_unflatten256 _rhs)
+        wpolylvec_bmul_irng (lvec_unflatten256 _lhs) /\
+        wpolylvec_bmul_irng (lvec_unflatten256 _rhs)
         ==>
         lifts_wpoly res = ntt_dotp (lifts_wpolylvec (lvec_unflatten256 _lhs))
                                     (lifts_wpolylvec (lvec_unflatten256 _rhs))
     ].
 proof.
-admitted.
+have lvec_val := mldsa65_lvec.
+proc.
+while (0 <= i <= 5 /\ lhs = _lhs /\ rhs = _rhs /\
+       wpolylvec_bmul_irng (lvec_unflatten256 _lhs) /\
+       wpolylvec_bmul_irng (lvec_unflatten256 _rhs) /\
+       lifts_wpoly output =
+         dotp_partial (lifts_wpolylvec (lvec_unflatten256 _lhs))
+                      (lifts_wpolylvec (lvec_unflatten256 _rhs)) i /\
+       wpoly_srng (i * (q-1)) (i * (q-1)) output
+      ); last first.
++ (* Exit + pre-loop: zero then initial invariant *)
+  wp; ecall (polynomial____zero_correct output). wp.
+  auto => /> Hbmul_lhs Hbmul_rhs result Hzero Hsrng; split.
+  + (* Initial invariant at i=0: lifts of zero = dotp_partial 0 *)
+    rewrite /dotp_partial /= /lifts_wpoly /poly_zero.
+    apply Array256.tP => j jb.
+    rewrite mapiE; 1: smt().
+    rewrite /= Hzero; 1: smt().
+    by rewrite (iota0 0 0) //= /create initiE 1:/# /= /to_sint /= /smod /= /zero.
+  + (* Exit: i=5, dotp_partial 5 = ntt_dotp *)
+    move => i0 out0 Hng Hi1 Hi2 Hlifts Hsrng0.
+    rewrite Hlifts; have -> : i0 = lvec by smt(mldsa65_lvec).
+    by rewrite dotp_partial_ntt_dotp.
+(* Loop body: pmmar then add_to_total *)
+wp; ecall (polynomial____pointwise_add_to_total_correct output product (i * (q-1)) (q-1)).
+ecall (polynomial__pointwise_montgomery_multiply_and_reduce_correct
+         product
+         (Array256.init (fun j => lhs.[(256 * i) + j]))
+         (Array256.init (fun j => rhs.[(256 * i) + j]))).
+auto => /> &hr Hi1 Hi2 Hbmul_lhs Hbmul_rhs Hlifts Hsrng Hguard.
+split.
++ (* bmul preconditions *)
+  split.
+  - have /= Heq_lhs := lvec_slice_eq _lhs (256 * i{hr}) _ _; 1,2: smt().
+    rewrite -Heq_lhs.
+    by move: Hbmul_lhs; rewrite /wpolylvec_bmul_irng LArray.allP => H; apply H; smt().
+  - have /= Heq_rhs := lvec_slice_eq _rhs (256 * i{hr}) _ _; 1,2: smt().
+    rewrite -Heq_rhs.
+    by move: Hbmul_rhs; rewrite /wpolylvec_bmul_irng LArray.allP => H; apply H; smt().
++ (* continuation after pmmar *)
+  move => _ _ product Hbmul_eq Hbmul_rng; split; 1: smt().
+  move => Hoverflow result0 Hadd_eq Hadd_rng.
+  do split; 1,2: smt().
+  + (* lifts: dotp_partial at i+1 *)
+    have Hlhs_slice : lifts_wpoly (init (fun j => _lhs.[n * i{hr} + j])) =
+        (lifts_wpolylvec (lvec_unflatten256 _lhs)).[i{hr}].
+    + rewrite /lifts_wpolylvec mapiE; 1: smt(mldsa65_lvec).
+      by rewrite -lvec_slice_eq; smt().
+    have Hrhs_slice : lifts_wpoly (init (fun j => _rhs.[n * i{hr} + j])) =
+        (lifts_wpolylvec (lvec_unflatten256 _rhs)).[i{hr}].
+    + rewrite /lifts_wpolylvec mapiE; 1: smt(mldsa65_lvec).
+      by rewrite -lvec_slice_eq; smt().
+    rewrite Hadd_eq Hlifts Hbmul_eq Hlhs_slice Hrhs_slice dotp_partialS; 1: smt().
+    pose a := dotp_partial _ _.
+    pose b := basemul _ _.
+    admit. (* TODO PY: &+ commutativity *)
+  + (* range: (i+1)*(q-1) *)
+    by have -> : (i{hr} + 1) * (q - 1) = i{hr} * (q - 1) + (q - 1) by ring.
+qed.
 
 lemma row_vector____dot_product_ph
       (_out : W32.t Array256.t)
       (_lhs : W32.t Array1280.t) (_rhs : W32.t Array1280.t) :
     phoare [ M.row_vector____dot_product :
         output = _out /\ lhs = _lhs /\ rhs = _rhs /\
-        wpolylvec_ntt_orng (lvec_unflatten256 _lhs) /\
-        wpolylvec_ntt_orng (lvec_unflatten256 _rhs)
+        wpolylvec_bmul_irng (lvec_unflatten256 _lhs) /\
+        wpolylvec_bmul_irng (lvec_unflatten256 _rhs)
         ==>
         lifts_wpoly res = ntt_dotp (lifts_wpolylvec (lvec_unflatten256 _lhs))
                                     (lifts_wpolylvec (lvec_unflatten256 _rhs))
@@ -146,8 +216,8 @@ lemma row_vector____multiply_with_matrix_A_correct
       (_mat : W32.t Array7680.t) (_vec : W32.t Array1280.t) :
     hoare [ M.row_vector____multiply_with_matrix_A :
         matrix_A = _mat /\ vector = _vec /\
-        wpolylvec_ntt_orng (lvec_unflatten256 _vec)
-        (* matrix_A range: each row is a polylvec with ntt_orng *)
+        wpolylvec_bmul_irng (lvec_unflatten256 _vec)
+        (* matrix_A range: each row is a polylvec with bmul_irng *)
         ==>
         lifts_wpolykvec (kvec_unflatten256 res) =
           ntt_mulmxv (liftu_wpolymat (mat_unflatten256 _mat))
@@ -160,7 +230,7 @@ lemma row_vector____multiply_with_matrix_A_ph
       (_mat : W32.t Array7680.t) (_vec : W32.t Array1280.t) :
     phoare [ M.row_vector____multiply_with_matrix_A :
         matrix_A = _mat /\ vector = _vec /\
-        wpolylvec_ntt_orng (lvec_unflatten256 _vec)
+        wpolylvec_bmul_irng (lvec_unflatten256 _vec)
         ==>
         lifts_wpolykvec (kvec_unflatten256 res) =
           ntt_mulmxv (liftu_wpolymat (mat_unflatten256 _mat))
